Change the style of agility

specs/Spec.Blake2.fst
@@ -7,21 +7,30 @@ open Lib.Sequence
 open Lib.ByteSequence
 open Lib.LoopCombinators
 
+#set-options "--z3rlimit 25 --max_fuel 0"
 
-noeq type parameters =
-  | MkParameters:
-    wt:inttype{wt = U32 \/ wt = U64} ->
-    rounds:size_nat ->
-    rTable:lseq (rotval wt) 4 ->
-    ivTable:lseq (uint_t wt) 8 ->
-    parameters
+type alg =
+  | Blake2S
+  | Blake2B
+
+inline_for_extraction
+let wt (a:alg) =
+  match a with
+  | Blake2S -> U32
+  | Blake2B -> U64
+
+inline_for_extraction
+let rounds (a:alg) =
+  match a with
+  | Blake2S -> 10
+  | Blake2B -> 12
 
 
 (* Algorithm parameters *)
 inline_for_extraction let size_hash_w : size_nat = 8
 inline_for_extraction let size_block_w : size_nat = 16
-inline_for_extraction let size_word (p:parameters) : size_nat = numbytes p.wt
-inline_for_extraction let size_block (p:parameters) : size_nat = size_block_w * (size_word p)
+inline_for_extraction let size_word (a:alg) : size_nat = numbytes (wt a)
+inline_for_extraction let size_block (a:alg) : size_nat = size_block_w * (size_word a)
 inline_for_extraction let max_size_hash : size_nat = 32
 
 inline_for_extraction let size_const_iv : size_nat = 8
@@ -30,47 +39,81 @@ inline_for_extraction let size_const_sigma : size_nat = 160
 
 (* Definition of base types *)
 inline_for_extraction
-let limb_inttype (p:parameters) =
-  match p.wt with
+let limb_inttype (a:alg) =
+  match (wt a) with
   | U32 -> U64
   | U64 -> U128
 
-type word_t (p:parameters) = uint_t p.wt
-type limb_t (p:parameters) : Type0 = uint_t (limb_inttype p)
+type word_t (a:alg) = uint_t (wt a)
+type limb_t (a:alg) : Type0 = uint_t (limb_inttype a)
 
-let to_word (p:parameters) (x:size_nat) : word_t p =
-  match p.wt with
+inline_for_extraction
+let to_word (a:alg) (x:size_nat) : word_t a =
+  match (wt a) with
   | U32 -> u32 x
   | U64 -> u64 x
 
-let to_limb (p:parameters) (x:size_nat) : limb_t p =
-  match p.wt with
+inline_for_extraction
+let to_limb (a:alg) (x:size_nat) : limb_t a =
+  match (wt a) with
   | U32 -> u64 x
   | U64 -> u128 x
 
-let limb_to_word (p:parameters) (x:limb_t p) : word_t p =
-  match p.wt with
+inline_for_extraction
+let limb_to_word (a:alg) (x:limb_t a) : word_t a =
+  match (wt a) with
   | U32 -> to_u32 #U64 x
   | U64 -> to_u64 #U128 x
 
 
-type working_vector_s (p:parameters) = lseq (word_t p) size_block_w
-type message_block_ws (p:parameters) = lseq (word_t p) size_block_w
-type message_block_s (p:parameters) = lseq uint8 (size_block p)
-type hash_state_s (p:parameters) = lseq (word_t p) size_hash_w
-type idx_t = n:size_nat{n < 16}
-type last_block_flag = bool
-
 
 inline_for_extraction
-let const_FF (p:parameters) : word_t p =
-  match p.wt with
-  | U32 -> u32 0xFFFFFFFF
-  | U64 -> u64 0xFFFFFFFFFFFFFFFF
+let rTable_list_S : l:list (rotval U32){List.Tot.length l = 4} =
+  [
+    size 16; size 12; size 8; size 7
+  ]
+
+inline_for_extraction
+let rTable_list_B: l:list (rotval U64){List.Tot.length l = 4} =
+  [
+    size 32; size 24; size 16; size 63
+  ]
+
+inline_for_extraction
+let rTable (a:alg) : lseq (rotval (wt a)) 4 =
+  match a with
+  | Blake2S -> of_list rTable_list_S
+  | Blake2B -> of_list rTable_list_B
 
 
-type list_sigma_elt_t = n:size_t{size_v n < 16}
-type list_sigma_t = l:list list_sigma_elt_t{List.Tot.length l <= max_size_t}
+inline_for_extraction let list_iv_S: l:list uint32{List.Tot.length l = 8} =
+  [@inline_let]
+  let l =
+  [u32 0x6A09E667; u32 0xBB67AE85; u32 0x3C6EF372; u32 0xA54FF53A;
+   u32 0x510E527F; u32 0x9B05688C; u32 0x1F83D9AB; u32 0x5BE0CD19] in
+  assert_norm(List.Tot.length l = 8);
+  l
+
+inline_for_extraction let list_iv_B: l:list uint64{List.Tot.length l = 8}  =
+  [@inline_let]
+  let l = [
+    u64 0x6A09E667F3BCC908; u64 0xBB67AE8584CAA73B;
+    u64 0x3C6EF372FE94F82B; u64 0xA54FF53A5F1D36F1;
+    u64 0x510E527FADE682D1; u64 0x9B05688C2B3E6C1F;
+    u64 0x1F83D9ABFB41BD6B; u64 0x5BE0CD19137E2179]
+  in
+  assert_norm(List.Tot.length l = 8);
+  l
+
+inline_for_extraction
+let ivTable (a:alg) : lseq (word_t a) 8 =
+  match a with
+  | Blake2S -> of_list list_iv_S
+  | Blake2B -> of_list list_iv_B
+
+type sigma_elt_t = n:size_t{size_v n < 16}
+type list_sigma_t = l:list sigma_elt_t{List.Tot.length l = 160}
+
 inline_for_extraction let list_sigma: list_sigma_t =
   [@inline_let]
   let l = [
@@ -95,106 +138,122 @@ inline_for_extraction let list_sigma: list_sigma_t =
     size 10; size  2; size  8; size  4; size  7; size  6; size  1; size  5;
     size 15; size 11; size  9; size 14; size  3; size 12; size 13; size  0]
   in
-  assert_norm(List.Tot.length l <= max_size_t);
+  assert_norm(List.Tot.length l = 160);
   l
 
-let const_sigma:lseq (n:size_t{size_v n < 16}) size_const_sigma =
+let const_sigma:lseq sigma_elt_t size_const_sigma =
   assert_norm (List.Tot.length list_sigma = size_const_sigma);
   of_list list_sigma
 
 
-(* Functions *)
-let g1 (p:parameters) (wv:working_vector_s p) (a:idx_t) (b:idx_t) (r:rotval p.wt) : Tot (working_vector_s p) =
-  wv.[a] <- (wv.[a] ^. wv.[b]) >>>. r
+inline_for_extraction
+let const_FF (a:alg) : word_t a =
+  match (wt a) with
+  | U32 -> u32 0xFFFFFFFF
+  | U64 -> u64 0xFFFFFFFFFFFFFFFF
 
-let g2 (p:parameters) (wv:working_vector_s p) (a:idx_t) (b:idx_t) (x:word_t p) : Tot (working_vector_s p) =
-  wv.[a] <- (wv.[a] +. wv.[b] +. x)
+
+(* Algorithms types *)
+type working_vector_s (a:alg) = lseq (word_t a) size_block_w
+type message_block_ws (a:alg) = lseq (word_t a) size_block_w
+type message_block_s (a:alg) = lseq uint8 (size_block a)
+type hash_state_s (a:alg) = lseq (word_t a) size_hash_w
+type idx_t = n:size_nat{n < 16}
+type last_block_flag = bool
+
+
+(* Functions *)
+let g1 (a:alg) (wv:working_vector_s a) (i:idx_t) (j:idx_t) (r:rotval (wt a)) : Tot (working_vector_s a) =
+  wv.[i] <- (wv.[i] ^. wv.[j]) >>>. r
+
+let g2 (a:alg) (wv:working_vector_s a) (i:idx_t) (j:idx_t) (x:word_t a) : Tot (working_vector_s a) =
+  wv.[i] <- (wv.[i] +. wv.[j] +. x)
 
 val blake2_mixing:
-  p:parameters
-  -> ws:working_vector_s p
+  a:alg
+  -> ws:working_vector_s a
   -> idx_t
   -> idx_t
   -> idx_t
   -> idx_t
-  -> word_t p
-  -> word_t p ->
-  Tot (working_vector_s p)
+  -> word_t a
+  -> word_t a ->
+  Tot (working_vector_s a)
 
-let blake2_mixing p wv a b c d x y =
-  let wv = g2 p wv a b x in
-  let wv = g1 p wv d a p.rTable.[0] in
-  let wv = g2 p wv c d (to_word p 0) in
-  let wv = g1 p wv b c p.rTable.[1] in
-  let wv = g2 p wv a b y in
-  let wv = g1 p wv d a p.rTable.[2] in
-  let wv = g2 p wv c d (to_word p 0) in
-  let wv = g1 p wv b c p.rTable.[3] in
+let blake2_mixing al wv a b c d x y =
+  let wv = g2 al wv a b x in
+  let wv = g1 al wv d a (rTable al).[0] in
+  let wv = g2 al wv c d (to_word al 0) in
+  let wv = g1 al wv b c (rTable al).[1] in
+  let wv = g2 al wv a b y in
+  let wv = g1 al wv d a (rTable al).[2] in
+  let wv = g2 al wv c d (to_word al 0) in
+  let wv = g1 al wv b c (rTable al).[3] in
   wv
 
 
 val blake2_round1:
-    p:parameters
-  -> wv:working_vector_s p
-  -> m:message_block_ws p
+    a:alg
+  -> wv:working_vector_s a
+  -> m:message_block_ws a
   -> i:size_nat ->
-  Tot (working_vector_s p)
+  Tot (working_vector_s a)
 
-let blake2_round1 p wv m i =
+let blake2_round1 a wv m i =
   let s = sub const_sigma ((i % 10) * 16) 16 in
-  let wv = blake2_mixing p wv 0 4  8 12 (m.[size_v s.[ 0]]) (m.[size_v s.[ 1]]) in
-  let wv = blake2_mixing p wv 1 5  9 13 (m.[size_v s.[ 2]]) (m.[size_v s.[ 3]]) in
-  let wv = blake2_mixing p wv 2 6 10 14 (m.[size_v s.[ 4]]) (m.[size_v s.[ 5]]) in
-  let wv = blake2_mixing p wv 3 7 11 15 (m.[size_v s.[ 6]]) (m.[size_v s.[ 7]]) in
+  let wv = blake2_mixing a wv 0 4  8 12 (m.[size_v s.[ 0]]) (m.[size_v s.[ 1]]) in
+  let wv = blake2_mixing a wv 1 5  9 13 (m.[size_v s.[ 2]]) (m.[size_v s.[ 3]]) in
+  let wv = blake2_mixing a wv 2 6 10 14 (m.[size_v s.[ 4]]) (m.[size_v s.[ 5]]) in
+  let wv = blake2_mixing a wv 3 7 11 15 (m.[size_v s.[ 6]]) (m.[size_v s.[ 7]]) in
   wv
 
 
 val blake2_round2:
-    p:parameters
-  -> wv:working_vector_s p
-  -> m:message_block_ws p
+    a:alg
+  -> wv:working_vector_s a
+  -> m:message_block_ws a
   -> i:size_nat ->
-  Tot (working_vector_s p)
+  Tot (working_vector_s a)
 
-let blake2_round2 p wv m i =
+let blake2_round2 a wv m i =
   let s = sub const_sigma ((i % 10) * 16) 16 in
-  let wv = blake2_mixing p wv 0 5 10 15 (m.[size_v s.[ 8]]) (m.[size_v s.[ 9]]) in
-  let wv = blake2_mixing p wv 1 6 11 12 (m.[size_v s.[10]]) (m.[size_v s.[11]]) in
-  let wv = blake2_mixing p wv 2 7  8 13 (m.[size_v s.[12]]) (m.[size_v s.[13]]) in
-  let wv = blake2_mixing p wv 3 4  9 14 (m.[size_v s.[14]]) (m.[size_v s.[15]]) in
+  let wv = blake2_mixing a wv 0 5 10 15 (m.[size_v s.[ 8]]) (m.[size_v s.[ 9]]) in
+  let wv = blake2_mixing a wv 1 6 11 12 (m.[size_v s.[10]]) (m.[size_v s.[11]]) in
+  let wv = blake2_mixing a wv 2 7  8 13 (m.[size_v s.[12]]) (m.[size_v s.[13]]) in
+  let wv = blake2_mixing a wv 3 4  9 14 (m.[size_v s.[14]]) (m.[size_v s.[15]]) in
   wv
 
 
 val blake2_round:
-    p:parameters
-  -> m:message_block_ws p
+    a:alg
+  -> m:message_block_ws a
   -> i:size_nat
-  -> wv:working_vector_s p ->
-  Tot (working_vector_s p)
+  -> wv:working_vector_s a ->
+  Tot (working_vector_s a)
 
-let blake2_round p m i wv =
-  let wv = blake2_round1 p wv m i in
-  let wv = blake2_round2 p wv m i in
+let blake2_round a m i wv =
+  let wv = blake2_round1 a wv m i in
+  let wv = blake2_round2 a wv m i in
   wv
 
 
 val blake2_compress1:
-  p:parameters
-  -> wv:working_vector_s p
-  -> s:hash_state_s p
-  -> m:message_block_ws p
-  -> offset:limb_t p
+  a:alg
+  -> wv:working_vector_s a
+  -> s:hash_state_s a
+  -> m:message_block_ws a
+  -> offset:limb_t a
   -> flag:last_block_flag ->
-  Tot (working_vector_s p)
+  Tot (working_vector_s a)
 
-let blake2_compress1 p wv s m offset flag =
+let blake2_compress1 a wv s m offset flag =
   let wv = update_sub wv 0 8 s in
-  let wv = update_sub wv 8 8 p.ivTable in
-  let low_offset = limb_to_word p offset in
-  let high_offset = limb_to_word p (shift_right #(limb_inttype p) offset (size (bits p.wt))) in
+  let wv = update_sub wv 8 8 (ivTable a) in
+  let low_offset = limb_to_word a offset in
+  let high_offset = limb_to_word a (shift_right #(limb_inttype a) offset (size (bits (wt a)))) in
   let wv_12 = wv.[12] ^. low_offset in
   let wv_13 = wv.[13] ^. high_offset in
-  let wv_14 = wv.[14] ^. (const_FF p) in
+  let wv_14 = wv.[14] ^. (const_FF a) in
   let wv = wv.[12] <- wv_12 in
   let wv = wv.[13] <- wv_13 in
   let wv = if flag then wv.[14] <- wv_14 else wv in
@@ -202,228 +261,194 @@ let blake2_compress1 p wv s m offset flag =
 
 
 val blake2_compress2:
-    p:parameters
-  -> wv:working_vector_s p
-  -> m:message_block_ws p ->
-  Tot (working_vector_s p)
+    a:alg
+  -> wv:working_vector_s a
+  -> m:message_block_ws a ->
+  Tot (working_vector_s a)
 
-let blake2_compress2 p wv m = repeati p.rounds (blake2_round p m) wv
+let blake2_compress2 a wv m = repeati (rounds a) (blake2_round a m) wv
 
 
 val blake2_compress3_inner:
-  p:parameters
-  -> ws:working_vector_s p
+  a:alg
+  -> ws:working_vector_s a
   -> i:size_nat{i < 8}
-  -> s:hash_state_s p ->
-  Tot (hash_state_s p)
+  -> s:hash_state_s a ->
+  Tot (hash_state_s a)
 
-let blake2_compress3_inner p wv i s =
+let blake2_compress3_inner a wv i s =
   let i_plus_8 = i + 8 in
-  let si_xor_wvi = logxor #p.wt s.[i] wv.[i] in
-  let si = logxor #p.wt si_xor_wvi wv.[i_plus_8] in
+  let si_xor_wvi = logxor #(wt a) s.[i] wv.[i] in
+  let si = logxor #(wt a) si_xor_wvi wv.[i_plus_8] in
   s.[i] <- si
 
 
 val blake2_compress3:
-  p:parameters
-  -> ws:working_vector_s p
-  -> s:hash_state_s p ->
-  Tot (hash_state_s p)
+  a:alg
+  -> ws:working_vector_s a
+  -> s:hash_state_s a ->
+  Tot (hash_state_s a)
 
-let blake2_compress3 p wv s = repeati 8 (blake2_compress3_inner p wv) s
+let blake2_compress3 a wv s = repeati 8 (blake2_compress3_inner a wv) s
 
 
 val blake2_compress:
-    p:parameters
-  -> s:hash_state_s p
-  -> m:message_block_ws p
-  -> offset:limb_t p
+    a:alg
+  -> s:hash_state_s a
+  -> m:message_block_ws a
+  -> offset:limb_t a
   -> last_block_flag ->
-  Tot (hash_state_s p)
+  Tot (hash_state_s a)
 
-let blake2_compress p s m offset flag =
-  let wv = create 16 (to_word p 0) in
-  let wv = blake2_compress1 p wv s m offset flag in
-  let wv = blake2_compress2 p wv m in
-  let s = blake2_compress3 p wv s in
+let blake2_compress a s m offset flag =
+  let wv = create 16 (to_word a 0) in
+  let wv = blake2_compress1 a wv s m offset flag in
+  let wv = blake2_compress2 a wv m in
+  let s = blake2_compress3 a wv s in
   s
 
-val blake2s_update_block:
-    p:parameters
-  -> dd_prev:size_nat{(dd_prev + 1) * (size_block p) <= max_size_t}
-  -> d:message_block_s p
-  -> s:hash_state_s p ->
-  Tot (hash_state_s p)
+val blake2_update_block:
+    a:alg
+  -> dd_prev:size_nat{(dd_prev + 1) * (size_block a) <= max_size_t}
+  -> d:message_block_s a
+  -> s:hash_state_s a ->
+  Tot (hash_state_s a)
 
-let blake2s_update_block p dd_prev d s =
-//  assert (length d == 16 * 4);
-  let to_compress : lseq (word_t p) 16 = uints_from_bytes_le #p.wt #16 d in
-  let offset = to_limb p ((dd_prev + 1) * (size_block p)) in
-  blake2_compress p s to_compress offset false
-
-
-val blake2s_init_iv: p:parameters -> Tot (hash_state_s p)
-let blake2s_init_iv p = p.ivTable
+let blake2_update_block a dd_prev d s =
+  let to_compress : lseq (word_t a) 16 = uints_from_bytes_le #(wt a) #16 d in
+  let offset = to_limb a ((dd_prev + 1) * (size_block a)) in
+  blake2_compress a s to_compress offset false
 
 
-val blake2s_init_hash:
-    p:parameters
-  -> s:hash_state_s p
+val blake2_init_iv: a:alg -> Tot (hash_state_s a)
+let blake2_init_iv a = (ivTable a)
+
+
+val blake2_init_hash:
+    a:alg
+  -> s:hash_state_s a
   -> kk:size_nat{kk <= 32}
   -> nn:size_nat{1 <= nn /\ nn <= 32} ->
-  Tot (hash_state_s p)
+  Tot (hash_state_s a)
 
-let blake2s_init_hash p s kk nn =
+let blake2_init_hash a s kk nn =
   let s0 = s.[0] in
-  let s0' = s0 ^. (to_word p 0x01010000) ^. ((to_word p kk) <<. (size 8)) ^. (to_word p nn) in
+  let s0' = s0 ^. (to_word a 0x01010000) ^. ((to_word a kk) <<. (size 8)) ^. (to_word a nn) in
   s.[0] <- s0'
 
 
-val blake2s_init:
-    p:parameters
+val blake2_init:
+    a:alg
   -> kk:size_nat{kk <= 32}
   -> k:lbytes kk
   -> nn:size_nat{1 <= nn /\ nn <= 32} ->
-  Tot (hash_state_s p)
+  Tot (hash_state_s a)
 
-let blake2s_init p kk k nn =
-  let s = blake2s_init_iv p in
-  let s = blake2s_init_hash p s kk nn in
+let blake2_init a kk k nn =
+  let s = blake2_init_iv a in
+  let s = blake2_init_hash a s kk nn in
   if kk = 0 then s
   else begin
-    let key_block = create (size_block p) (u8 0) in
+    let key_block = create (size_block a) (u8 0) in
     let key_block = update_sub key_block 0 kk k in
-    blake2s_update_block p 0 key_block s end
+    blake2_update_block a 0 key_block s end
 
 
-val blake2s_update_multi_iteration:
-  p:parameters
+val blake2_update_multi_iteration:
+  a:alg
   -> dd_prev:size_nat
-  -> dd:size_nat{(dd + dd_prev) * (size_block p) <= max_size_t}
-  -> d:lbytes (dd * (size_block p))
+  -> dd:size_nat{(dd + dd_prev) * (size_block a) <= max_size_t}
+  -> d:lbytes (dd * (size_block a))
   -> i:size_nat{i + 1 <= dd}
-  -> s:hash_state_s p ->
-  Tot (hash_state_s p)
+  -> s:hash_state_s a ->
+  Tot (hash_state_s a)
 
-let blake2s_update_multi_iteration p dd_prev dd d i s =
-  let block = (sub d (i * (size_block p)) (size_block p)) in
-  blake2s_update_block p (dd_prev + i) block s
+let blake2_update_multi_iteration a dd_prev dd d i s =
+  let block = (sub d (i * (size_block a)) (size_block a)) in
+  blake2_update_block a (dd_prev + i) block s
 
 
-val blake2s_update_multi:
-    p:parameters
+val blake2_update_multi:
+    a:alg
   -> dd_prev:size_nat
-  -> dd:size_nat{(dd + dd_prev) * (size_block p) <= max_size_t}
-  -> d:lbytes (dd * (size_block p))
-  -> s:hash_state_s p ->
-  Tot (hash_state_s p)
+  -> dd:size_nat{(dd + dd_prev) * (size_block a) <= max_size_t}
+  -> d:lbytes (dd * (size_block a))
+  -> s:hash_state_s a ->
+  Tot (hash_state_s a)
 
-let blake2s_update_multi p dd_prev dd d s =
-  repeati dd (blake2s_update_multi_iteration p dd_prev dd d) s
+let blake2_update_multi a dd_prev dd d s =
+  repeati dd (blake2_update_multi_iteration a dd_prev dd d) s
 
 
-val blake2s_update_last_block:
-    p:parameters
-  -> ll:size_nat{ll + (size_block p) <= max_size_t}
-  -> last_block:lbytes (size_block p)
+val blake2_update_last_block:
+    a:alg
+  -> ll:size_nat{ll + (size_block a) <= max_size_t}
+  -> last_block:lbytes (size_block a)
   -> flag_key:bool
-  -> s:hash_state_s p ->
-  Tot (hash_state_s p)
+  -> s:hash_state_s a ->
+  Tot (hash_state_s a)
 
-let blake2s_update_last_block p ll last_block fk s =
-  let last_block : lseq (word_t p) 16 = uints_from_bytes_le #p.wt last_block in
+let blake2_update_last_block a ll last_block fk s =
+  let last_block : lseq (word_t a) 16 = uints_from_bytes_le #(wt a) last_block in
   if not fk then
-    blake2_compress p s last_block (to_limb p ll) true
+    blake2_compress a s last_block (to_limb a ll) true
   else
-    blake2_compress p s last_block (to_limb p (ll + (size_block p))) true
+    blake2_compress a s last_block (to_limb a (ll + (size_block a))) true
 
 
-val blake2s_update_last:
-    p:parameters
-  -> ll:size_nat{ll + (size_block p) <= max_size_t}
-  -> len:size_nat{len <= (size_block p)}
+val blake2_update_last:
+    a:alg
+  -> ll:size_nat{ll + (size_block a) <= max_size_t}
+  -> len:size_nat{len <= (size_block a)}
   -> last:lbytes len
   -> flag_key:bool
-  -> s:hash_state_s p ->
-  Tot (hash_state_s p)
+  -> s:hash_state_s a ->
+  Tot (hash_state_s a)
 
-let blake2s_update_last p ll len last fk s =
-  let last_block = create (size_block p) (u8 0) in
+let blake2_update_last a ll len last fk s =
+  let last_block = create (size_block a) (u8 0) in
   let last_block = update_sub last_block 0 len last in
-  blake2s_update_last_block p ll last_block fk s
+  blake2_update_last_block a ll last_block fk s
 
 
-val blake2s_update_last_empty: p:parameters -> s:hash_state_s p -> Tot (hash_state_s p)
-let blake2s_update_last_empty p st =
-  let data = create (size_block p) (u8 0) in
-  blake2s_update_last p 0 (size_block p) data false st
+val blake2_update_last_empty: a:alg -> s:hash_state_s a -> Tot (hash_state_s a)
+let blake2_update_last_empty a st =
+  let data = create (size_block a) (u8 0) in
+  blake2_update_last a 0 (size_block a) data false st
 
 
-val blake2s_finish:
-    p:parameters
-  -> s:hash_state_s p
+val blake2_finish:
+    a:alg
+  -> s:hash_state_s a
   -> nn:size_nat{1 <= nn /\ nn <= 32} ->
   Tot (lbytes nn)
 
-let blake2s_finish p s nn =
+let blake2_finish a s nn =
   let full = uints_to_bytes_le s in
   sub full 0 nn
 
 
-val blake2s:
-    p:parameters
-  -> ll:size_nat{ll + 2 * (size_block p) <= max_size_t} // This could be relaxed
+val blake2:
+    a:alg
+  -> ll:size_nat{ll + 2 * (size_block a) <= max_size_t} // This could be relaxed
   -> d:lbytes ll
   -> kk:size_nat{kk <= 32}
   -> k:lbytes kk
   -> nn:size_nat{1 <= nn /\ nn <= 32} ->
   Tot (lbytes nn)
 
-let blake2s p ll d kk k nn =
+let blake2 a ll d kk k nn =
   let fk = if kk = 0 then false else true in
-  let rem = ll % (size_block p) in
-  let nblocks = ll / (size_block p) in
-  let blocks = sub d 0 (nblocks * (size_block p)) in
-  let last = sub d (nblocks * (size_block p)) rem in
-  let s = blake2s_init p kk k nn in
+  let rem = ll % (size_block a) in
+  let nblocks = ll / (size_block a) in
+  let blocks = sub d 0 (nblocks * (size_block a)) in
+  let last = sub d (nblocks * (size_block a)) rem in
+  let s = blake2_init a kk k nn in
   let s =
-    if ll = 0 && kk = 0 then blake2s_update_last_empty p s
+    if ll = 0 && kk = 0 then blake2_update_last_empty a s
     else begin
       let nprev = if kk = 0 then 0 else 1 in
-      let s = blake2s_update_multi p nprev nblocks blocks s in
-      blake2s_update_last p ll rem last fk s end in
-  blake2s_finish p s nn
+      let s = blake2_update_multi a nprev nblocks blocks s in
+      blake2_update_last a ll rem last fk s end in
+  blake2_finish a s nn
 
-
-
-
-
-///
-/// Instanciation
-///
-
-(* Constants *)
-inline_for_extraction
-let rTable_list_S = [
-  size 16; size 12; size 8; size 7
-]
-
-inline_for_extraction
-let rTable_list_B = [
-  size 32; size 24; size 16; size 63
-]
-
-inline_for_extraction let list_iv_S =
-  [@inline_let]
-  let l =
-  [u32 0x6A09E667; u32 0xBB67AE85; u32 0x3C6EF372; u32 0xA54FF53A;
-   u32 0x510E527F; u32 0x9B05688C; u32 0x1F83D9AB; u32 0x5BE0CD19] in
-  assert_norm(List.Tot.length l <= max_size_t);
-  l
-
-inline_for_extraction let list_iv_B =
-  List.Tot.map u64
-  [0x6A09E667F3BCC908; 0xBB67AE8584CAA73B;
-   0x3C6EF372FE94F82B; 0xA54FF53A5F1D36F1;
-   0x510E527FADE682D1; 0x9B05688C2B3E6C1F;
-   0x1F83D9ABFB41BD6B; 0x5BE0CD19137E2179]
